challenge 5 checkpoint

Dafny/AbstractNonInterferenceProof.s.dfy
@@ -11,9 +11,9 @@ abstract module AbstractNonInterferenceProof {
     predicate MiniSpec(s:LLVM_def.state, s':LLVM_def.state)
 
     predicate ModuloMiniSpec(code:lvm_code, s:LLVM_def.state, s':LLVM_def.state,stateSeqS:seq<state>){
-        && startAndEndState(s,s',stateSeqS) 
-        && ValidStateSeq(stateSeqS) 
-        && StateSeqEvalsCode(code,stateSeqS)
+        && BehaviorDescribedByStates(s,s',stateSeqS) 
+        && ValidBehavior(stateSeqS) 
+        && BehaviorEvalsCode(code,stateSeqS)
         && (forall i :: (i >=0 && i < |stateSeqS|-2) ==> !MiniSpec(stateSeqS[i],stateSeqS[i+1]))
     }
 
@@ -23,21 +23,74 @@ abstract module AbstractNonInterferenceProof {
         requires evalCode(code, s, s')
         requires evalCode(code', r, r')
         ensures forall stateSeqS:seq<state>, stateSeqR:seq<state> 
-                ::  (&& startAndEndState(s,s',stateSeqS) 
-                    && ValidStateSeq(stateSeqS) 
-                    && startAndEndState(r,r',stateSeqR) 
-                    && ValidStateSeq(stateSeqR)
+                ::  (&& BehaviorDescribedByStates(s,s',stateSeqS) 
+                    && ValidBehavior(stateSeqS) 
+                    && BehaviorDescribedByStates(r,r',stateSeqR) 
+                    && ValidBehavior(stateSeqR)
                     && ModuloMiniSpec(code,s,s',stateSeqS)) ==> lvm_state_eq(s',r')
 }
 
+abstract module UpdatedAbstractNonInterferenceProof {
+    import opened LLVM_def
+    import opened control_flow
+
+    // Describes/Excludes 'bad' behaviors in the Unpatched Code (ie preBehaviors)
+    predicate RemovedBehaviors(b:behavior)
+
+    // Describes/Excludes 'good' added behavior in Patched Code (ie postBehaviors)
+    // [TODO] fix :: This is a placeholder for now -- ie this allows all executions of the patched code
+    predicate AddedBehaviors(b:behavior)
+    {
+        false
+    }
+
+    // The MiniSpec is a predicate over a behavior (finite seq of states [s to s']) 
+    predicate MiniSpec(b:behaviors)
+    {
+        match b
+            case preBehavior(preB) => RemovedBehaviors(preB)
+            case postBehavior(postB) => AddedBehaviors(postB)
+    }
+
+    /*
+        for all behaviors, pre(unpatched) and post(patched), such that the following is true:
+            Both are a valid sequence of states
+            The preBehavior is a valid behavior of the unpatched code
+            The postBehavior is a valid behavior of the patched code
+            The starting states are the same
+            The preBehavior does not include any 'bad' behaviors as expressed in 'RemovedBehaviors'
+            **The postBehavior does not include any 'good' added behavior as expressed in 'AddedBehaviors'
+        Implies that:
+            the final states of both behaviors are the same
+    */
+    lemma nonInterference(preCode:lvm_code, postCode:lvm_code)
+        ensures forall pre:behavior, post:behavior ::
+                   (&& ValidBehavior(pre) 
+                    && ValidBehavior(post)  
+                    && BehaviorEvalsCode(preCode,pre) 
+                    && BehaviorEvalsCode(postCode,post)
+                    && pre[0] == post[0] 
+                    && !MiniSpec(preBehavior(pre))
+                    && !MiniSpec(postBehavior(post)))
+                    ==> lvm_state_eq(pre[|pre|-1],post[|post|-1])
+
+
+}
 
 
 /*
-    what is the MiniSpec?
-    MiniSpec is a single state predicate that describes incorrect behavior (that is supposedly fixed by the patch)
 
-        This would describe/preclude all exections where there is a state that enters a 'danger' or buggy state. but not 
-        > necessarily 'acts' on it
+
+    predicate ModuloMiniSpec(code:lvm_code,b:behaviors)
+    {
+        var behavior := getBehavior(b);
+        (ValidBehavior(behavior) && BehaviorEvalsCode(code,behavior)) ==> !MiniSpec(b)
+    }
+
+
+
+/////
+    MiniSpec is a predicate over a behavior (finite seq of states [s to s']) that describes an incorrect action
 
 /////
     MiniSpec is a two-state predicate (s,s') that describes both the incorrect behavior and that incorrect behavior 
@@ -45,5 +98,14 @@ abstract module AbstractNonInterferenceProof {
         
         This only reasons about the exections where a state s enters a 'danger' state *and* makes the 
         > corresponding transition 
+
+//////        
+    what is the MiniSpec?
+    MiniSpec is a single state predicate that describes incorrect behavior (that is supposedly fixed by the patch)
+
+        This would describe/preclude all exections where there is a state that enters a 'danger' or buggy state. but not 
+        > necessarily 'acts' on it
+
+
 */
     
