Dafny/LLVM/generalInstructionsBehavior.i.dfy
@@ -1,0 +1,875 @@
+include "./llvm.i.dfy"
+include "./control_flow.i.dfy"
+include "./types.dfy"
+include "./memory.i.dfy"
+include "./Operations/binaryOperations.i.dfy"
+include "./Operations/conversionOperations.i.dfy"
+include "./Operations/bitwiseBinaryOperations.i.dfy"
+include "./Operations/otherOperations.i.dfy"
+
+module general_instructions_behaviors {
+    import opened LLVM_def
+    import opened control_flow
+    import opened types
+    import opened memory
+    import opened binary_operations_i
+    import opened conversion_operations_i
+    import opened bitwise_binary_operations_i
+    import opened other_operations_i
+
+function method lvm_code_Add(dst:lvm_operand_opr, size:nat, src1:lvm_operand_opr,src2:lvm_operand_opr):lvm_code
+
+{
+   Ins(ADD(dst, size,src1,src2))
+}
+lemma lvm_lemma_Add_behavior(b:behavior,lvm_b0:lvm_codes, lvm_sN:lvm_state, 
+            dst:lvm_operand_opr, size:nat, src1:lvm_operand_opr,src2:lvm_operand_opr)
+  returns (b':behavior,lvm_bM:lvm_codes, lvm_sM:lvm_state)
+
+  requires ValidBehaviorNonTrivial(b);
+  requires lvm_require(lvm_b0, lvm_code_Add(dst, size,src1,src2), bls(b), lvm_sN)
+  requires lvm_is_dst_opr(dst, bls(b))
+  requires lvm_is_src_opr(src1, bls(b))
+  requires lvm_get_ok(bls(b))
+
+  requires ValidOperand(bls(b),src1);
+  requires OperandContents(bls(b),src1).Int?;
+  requires ValidOperand(bls(b),src2);
+  requires OperandContents(bls(b),src2).Int?;
+  requires ValidOperand(bls(b),dst);
+  // requires OperandContents(bls(b),dst).Int?;
+
+  requires typesMatch(OperandContents(bls(b),src1),OperandContents(bls(b),src2))
+  requires size == OperandContents(bls(b),src1).itype.size
+  requires lvm_code_Add(dst, size,src1,src2).Ins?;
+// //   
+  ensures  lvm_ensure(lvm_b0, lvm_bM, bls(b), lvm_sM, lvm_sN)
+  ensures  lvm_get_ok(lvm_sM)
+  ensures  ValidOperand(lvm_sM,dst)
+  ensures  ValidOperand(lvm_sM,src1)
+  ensures OperandContents(lvm_sM,src1).Int?;
+  ensures  ValidOperand(lvm_sM,src2)
+  ensures OperandContents(lvm_sM,src2).Int?;
+  ensures OperandContents(lvm_sM,dst).Int?;
+  ensures OperandContents(lvm_sM,dst).itype.size == size;
+  ensures !OperandContents(lvm_sM,dst).itype.signed
+
+
+  ensures  OperandContents(lvm_sM,dst).Int?;
+  ensures  lvm_state_eq(lvm_sM, lvm_update_mem( lvm_sM, lvm_update_all(lvm_sM, bls(b))))
+  ensures  lvm_state_eq(lvm_sM, lvm_update_ok(lvm_sM, lvm_update_all( lvm_sM, bls(b))))
+  ensures  forall s2 :: evalCode(lvm_b0.hd, bls(b), s2) ==> s2.ok
+    // ensures typesMatch(OperandContents(lvm_sM,src1),OperandContents(lvm_sM,src2))
+
+  // ensures OperandContents(lvm_sM, dst).val == evalADD(OperandContents(bls(b),dst).itype.size,OperandContents(bls(b),src1),OperandContents(bls(b),src2)).val;
+  ensures ToTwosComp(OperandContents(lvm_sM, dst)).val == 
+          (OperandContents(bls(b), src1).val + OperandContents(bls(b), src2).val) % Pow256(OperandContents(bls(b), src1).itype.size)
+  ensures forall d :: ValidOperand(bls(b),d) && d != dst ==> ValidOperand(lvm_sM,d) && OperandContents(bls(b),d) == OperandContents(lvm_sM,d)
+  ensures StateNext(bls(b),lvm_sM)
+  ensures ValidBehavior(b');
+{
+    var lvm_s0 := bls(b);
+    assert lvm_code_Add(dst, size,src1,src2).Ins?;
+    var addIns := lvm_code_Add(dst, size,src1,src2).ins;
+    assert ValidInstruction(lvm_s0,addIns);
+
+    assert  ValidRegOperand(lvm_s0, dst);
+    assert ValidState(lvm_s0);
+    var lvm_old_s:lvm_state := lvm_s0;
+    assert evalCode_lax(lvm_Block(lvm_b0), lvm_s0, lvm_sN);
+    assert lvm_s0.ok;
+    assert eval_code(lvm_Block(lvm_b0), lvm_s0, lvm_sN);
+    assert evalBlock(lvm_Block(lvm_b0).block, lvm_s0, lvm_sN);
+    assert exists r' :: (evalCode(lvm_b0.hd, lvm_s0, r'));
+
+    ghost var lvm_ltmp1, lvm_cM:lvm_code, lvm_ltmp2 := lvm_lemma_block(lvm_b0, lvm_s0, lvm_sN);
+    lvm_sM := lvm_ltmp1;
+    lvm_bM := lvm_ltmp2;
+    assert lvm_b0.tl == lvm_bM;
+    assert ValidState(lvm_s0);
+    assert lvm_s0.ok;
+    assert ValidState(lvm_sM);
+    assert ValidOperand(lvm_sM,dst);
+    assert evalIns(lvm_code_Add(dst, size,src1,src2).ins,lvm_s0,lvm_sM);
+    assert NextStep(lvm_s0,lvm_sM,evalInsStep(lvm_code_Add(dst, size,src1,src2).ins));
+    assert MemStateNext(lvm_s0.m,lvm_sM.m,MemStep.stutterStep());
+    assert StateNext(lvm_s0,lvm_sM);
+    b' := b + [lvm_sM];
+    assert ValidBehavior(b');
+    assert BehaviorEvalsCode(lvm_code_Add(dst, size,src1,src2),[lvm_s0,lvm_sM]);
+    // var evalA := evalADD(OperandContents(lvm_s0,dst).itype.size,OperandContents(lvm_s0,src1),OperandContents(lvm_s0,src2));
+    // assert evalUpdate(lvm_s0, dst, evalA,lvm_sM);
+    assert (forall d :: ValidOperand(lvm_s0,d) && d != dst ==> ValidOperand(lvm_sM,d) && OperandContents(lvm_s0,d) == OperandContents(lvm_sM,d));
+    // assert ValidData(lvm_sM,evalADD(OperandContents(lvm_s0,dst).itype.size,OperandContents(lvm_s0,src1),OperandContents(lvm_s0,src2)));
+    assert OperandContents(lvm_sM, dst).val == evalADD(OperandContents(lvm_s0,src1).itype.size,OperandContents(lvm_s0,src1),OperandContents(lvm_s0,src2)).val;
+}
+
+function method lvm_code_GetElementPtr(dst:lvm_operand_opr,t:bitWidth,op1:lvm_operand_opr,op2:lvm_operand_opr):lvm_code
+{
+    //getelementptr
+    
+    Ins(GETELEMENTPTR(dst,t,op1,op2))
+
+}
+
+lemma lvm_lemma_GetElementPtr(b:behavior,lvm_b0:lvm_codes, lvm_sN:lvm_state, 
+            dst:lvm_operand_opr,s:MemState,t:bitWidth,op1:lvm_operand_opr,op2:lvm_operand_opr)
+  returns (b':behavior,lvm_bM:lvm_codes, lvm_sM:lvm_state)
+  
+    requires ValidBehaviorNonTrivial(b);
+
+  requires lvm_require(lvm_b0, lvm_code_GetElementPtr(dst,t,op1,op2), bls(b), lvm_sN)
+  requires lvm_is_dst_opr(dst, bls(b))
+  requires lvm_is_src_opr(op1, bls(b))
+  requires lvm_get_ok(bls(b))
+
+  requires ValidOperand(bls(b),op1);
+  requires ValidOperand(bls(b),op2);
+  requires OperandContents(bls(b),op1).Ptr?;
+  requires OperandContents(bls(b),op2).Int?;
+  requires !OperandContents(bls(b),op2).itype.signed;
+  requires |bls(b).m.mem[OperandContents(bls(b),op1).bid]| == t
+
+  requires OperandContents(bls(b),op1).bid in bls(b).m.mem; //needed for IsValidBid for valid input
+  requires ValidOperand(bls(b),dst)
+//   
+ensures bls(b).m == lvm_sM.m;
+  ensures  lvm_ensure(lvm_b0, lvm_bM, bls(b), lvm_sM, lvm_sN)
+  ensures  lvm_get_ok(lvm_sM)
+  ensures ValidOperand(lvm_sM,dst)
+
+  ensures OperandContents(lvm_sM,dst).Ptr?;
+  ensures  OperandContents(lvm_sM, dst) == evalGETELEMENTPTR(bls(b).m,t,OperandContents(bls(b),op1),OperandContents(bls(b),op2));
+  ensures  lvm_state_eq(lvm_sM, lvm_update_ok(lvm_sM, lvm_update_all( lvm_sM, bls(b))))
+  ensures forall d :: ValidOperand(bls(b),d) && d != dst ==> ValidOperand(lvm_sM,d) && OperandContents(bls(b),d) == OperandContents(lvm_sM,d)
+  ensures StateNext(bls(b),lvm_sM)
+  ensures ValidBehavior(b');
+
+{ 
+  var lvm_s0 := bls(b);
+  assert evalBlock(lvm_b0, lvm_s0, lvm_sN);
+
+  ghost var lvm_ltmp1, lvm_cM:lvm_code, lvm_ltmp2 := lvm_lemma_block(lvm_b0, lvm_s0, lvm_sN);
+  lvm_sM := lvm_ltmp1;
+  lvm_bM := lvm_ltmp2;
+//   var lvm_b1:lvm_codes := lvm_get_block(lvm_cM);
+  assert lvm_sM.ok;
+  assert lvm_b0.tl == lvm_bM;
+
+  assert ValidState(lvm_sM);
+  assert evalCode_lax(lvm_cM, lvm_s0, lvm_sM);
+  assert NextStep(lvm_s0,lvm_sM,evalInsStep(lvm_code_GetElementPtr(dst,t,op1,op2).ins));
+  assert MemStateNext(lvm_s0.m,lvm_sM.m,MemStep.stutterStep());
+  b' := b + [lvm_sM];
+  assert ValidBehavior(b');
+  assert BehaviorEvalsCode(lvm_code_GetElementPtr(dst,t,op1,op2),[lvm_s0,lvm_sM]);
+
+}
+
+
+function method lvm_code_Ret(op1:lvm_operand_opr):lvm_code
+{
+    //getelementptr
+    
+    Ins(RET(op1))
+
+}
+
+lemma lvm_ret_behavior(b:behavior,lvm_b0:lvm_codes,lvm_sN:lvm_state,op1:lvm_operand_opr) 
+  returns (b':behavior, lvm_bM:lvm_codes, lvm_sM:lvm_state)
+  // requires code.Ins? && code.ins.RET?;
+  // requires ValidInstruction(lvm_s0,code.ins);
+  requires ValidBehaviorNonTrivial(b);
+  requires ValidState(bls(b));
+  requires lvm_require(lvm_b0, lvm_code_Ret(op1), bls(b), lvm_sN);
+  requires ValidOperand(bls(b),op1);
+  // requires lvm_s0 == bls(b);
+  ensures  lvm_ensure(lvm_b0, lvm_bM, bls(b), lvm_sM, lvm_sN)
+  ensures  lvm_get_ok(lvm_sM)
+  ensures  OperandContents(bls(b),op1).Void? ==> bls(b) == lvm_sM
+  ensures  lvm_state_eq(lvm_sM,  bls(b))
+  ensures lvm_bM == lvm_b0.tl;
+  // ensures forall d :: ValidOperand(bls(b),d) && d != dst ==> ValidOperand(lvm_sM,d) && OperandContents(bls(b),d) == OperandContents(lvm_sM,d)
+  ensures StateNext(bls(b),lvm_sM);
+  ensures ValidBehavior(b');
+
+{
+  // assert forall
+  // assert exists s' :: evalIns(code.ins,lvm_s0,s');
+  // var s' :| evalCode(code,lvm_s0,s');
+  var lvm_s0 := bls(b);
+  assert evalBlock(lvm_b0, lvm_s0, lvm_sN);
+
+  ghost var lvm_ltmp1, lvm_cM:lvm_code, lvm_ltmp2 := lvm_lemma_block(lvm_b0, lvm_s0, lvm_sN);
+    lvm_sM := lvm_ltmp1;
+    lvm_bM := lvm_ltmp2;
+
+  assert lvm_b0.tl == lvm_bM;
+
+  assert ValidState(lvm_sM);
+  assert evalCode(lvm_cM, lvm_s0, lvm_sM);
+  assert NextStep(lvm_s0,lvm_sM,evalInsStep(lvm_code_Ret(op1).ins));
+  assert MemStateNext(lvm_s0.m,lvm_sM.m,MemStep.stutterStep());
+  assert StateNext(lvm_s0,lvm_sM);
+
+  b' := b + [lvm_sM];
+  assert ValidBehavior(b');
+  assert BehaviorEvalsCode(lvm_code_Ret(op1),[lvm_s0,lvm_sM]);
+}
+
+lemma lvm_lemma_Ret(lvm_b0:lvm_codes, lvm_s0:lvm_state, lvm_sN:lvm_state,dst:lvm_operand_opr, op1:lvm_operand_opr)
+  returns (lvm_bM:lvm_codes, lvm_sM:lvm_state)
+  
+  requires lvm_require(lvm_b0, lvm_code_Ret(op1), lvm_s0, lvm_sN)
+  requires lvm_is_dst_opr(dst, lvm_s0)
+  requires lvm_is_src_opr(op1, lvm_s0)
+  requires lvm_get_ok(lvm_s0)
+
+  requires ValidOperand(lvm_s0,op1);
+
+//   
+  ensures  lvm_ensure(lvm_b0, lvm_bM, lvm_s0, lvm_sM, lvm_sN)
+  ensures  lvm_get_ok(lvm_sM)
+  ensures  OperandContents(lvm_s0,op1).Void? ==> lvm_s0 == lvm_sM
+  ensures  lvm_state_eq(lvm_sM,  lvm_s0)
+  ensures lvm_bM == lvm_b0.tl;
+  ensures forall d :: ValidOperand(lvm_s0,d) && d != dst ==> ValidOperand(lvm_sM,d) && OperandContents(lvm_s0,d) == OperandContents(lvm_sM,d)
+  ensures StateNext(lvm_s0,lvm_sM);
+
+{
+  
+  
+
+  assert evalBlock(lvm_b0, lvm_s0, lvm_sN);
+
+  ghost var lvm_ltmp1, lvm_cM:lvm_code, lvm_ltmp2 := lvm_lemma_block(lvm_b0, lvm_s0, lvm_sN);
+  lvm_sM := lvm_ltmp1;
+  lvm_bM := lvm_ltmp2;
+
+  assert lvm_b0.tl == lvm_bM;
+
+  assert ValidState(lvm_sM);
+  assert evalCode(lvm_cM, lvm_s0, lvm_sM);
+  assert NextStep(lvm_s0,lvm_sM,evalInsStep(lvm_code_Ret(op1).ins));
+  assert MemStateNext(lvm_s0.m,lvm_sM.m,MemStep.stutterStep());
+
+
+}
+
+
+function method lvm_LOAD(dst:lvm_operand_opr,t:bitWidth,op1:lvm_operand_opr):lvm_code
+{
+    
+    Ins(LOAD(dst,t,op1))
+}
+
+
+lemma lvm_lemma_Load(b:behavior,lvm_b0:lvm_codes, lvm_sN:lvm_state,dst:lvm_operand_opr,t:bitWidth,op1:lvm_operand_opr)
+  returns (b':behavior,lvm_bM:lvm_codes, lvm_sM:lvm_state)
+  requires ValidBehaviorNonTrivial(b);
+  requires lvm_require(lvm_b0, lvm_LOAD(dst,t,op1), bls(b), lvm_sN)
+  requires lvm_is_dst_opr(dst, bls(b))
+  requires lvm_is_src_opr(op1, bls(b))
+  requires lvm_get_ok(bls(b))
+
+  requires ValidOperand(bls(b),op1);
+  requires ValidOperand(bls(b),dst);
+  requires OperandContents(bls(b),op1).Ptr?;
+  requires MemValid(bls(b).m);
+  requires IsValidPtr(bls(b).m,OperandContents(bls(b),op1).bid,OperandContents(bls(b),op1).offset,t);
+  // requires bls(b).m == lvm_sN.m;
+//   
+  ensures  lvm_sM.ok ==> lvm_ensure(lvm_b0, lvm_bM, bls(b), lvm_sM, lvm_sN)
+  ensures  lvm_sM.ok ==> lvm_get_ok(lvm_sM)
+  ensures  lvm_sM.ok ==> ValidOperand(lvm_sM,dst);
+  ensures  lvm_sM.ok ==> !OperandContents(lvm_sM,dst).Ptr?;
+  ensures  lvm_sM.ok ==> OperandContents(lvm_sM,dst).Int?;
+
+  ensures lvm_sM.ok ==> OperandContents(lvm_sM,dst).Bytes? ==> validBitWidth(|OperandContents(lvm_sM,dst).bytes|)
+  ensures lvm_sM.ok ==> OperandContents(lvm_sM,dst).Int? || OperandContents(lvm_sM,dst).Bytes? || OperandContents(lvm_sM,dst).Void?;
+  ensures lvm_sM.ok ==> OperandContents(lvm_sM,dst).Int? ==> OperandContents(lvm_sM,dst).itype.size == t;
+  ensures bls(b).m == lvm_sM.m;
+  ensures lvm_sM.ok ==> forall d :: ValidOperand(bls(b),d) && d != dst ==> ValidOperand(lvm_sM,d) && OperandContents(bls(b),d) == OperandContents(lvm_sM,d)
+  ensures lvm_sM.ok ==> StateNext(bls(b),lvm_sM)
+  ensures ValidBehavior(b');
+
+{
+  
+  
+  
+  var lvm_s0 := bls(b);
+  assert evalBlock(lvm_b0, lvm_s0, lvm_sN);
+  assert lvm_s0.ok;
+  assert ValidInstruction(lvm_s0,lvm_b0.hd.ins);
+
+  assert IsValidPtr(lvm_s0.m, OperandContents(lvm_s0,lvm_b0.hd.ins.src).bid,OperandContents(lvm_s0,lvm_b0.hd.ins.src).offset,t);
+//   assert exists d:Data :: Load(lvm_s0.m,lvm_sN.m,OperandContents(lvm_s0,lvm_b0.hd.ins.src).bid,OperandContents(lvm_s0,lvm_b0.hd.ins.src).offset,d);
+  // assert lvm_s0.m == lvm_sN.m;
+//   assert exists d:Data :: Load(lvm_s0.m,lvm_sN.m,OperandContents(lvm_s0,lvm_b0.hd.ins.src).bid,OperandContents(lvm_s0,lvm_b0.hd.ins.src).offset,d); 
+//   assert lvm_s0.ok == lvm_sN.ok;
+
+
+  ghost var lvm_ltmp1, lvm_cM:lvm_code, lvm_ltmp2 := lvm_lemma_block(lvm_b0, lvm_s0, lvm_sN);
+  lvm_sM := lvm_ltmp1;
+  lvm_bM := lvm_ltmp2;
+ 
+  var d := evalLOAD(lvm_s0.m,lvm_sM.m,lvm_b0.hd.ins.t,OperandContents(lvm_s0,lvm_b0.hd.ins.src));
+  assert d == evalLOAD(lvm_s0.m,lvm_sM.m,lvm_b0.hd.ins.t,OperandContents(lvm_s0,lvm_b0.hd.ins.src));
+  assert D(d).D?;
+
+  // assert evalLOAD(lvm_s0.m,lvm_sM.m,lvm_b0.hd.ins.t,OperandContents(lvm_s0,lvm_b0.hd.ins.src)).Void? ==> !lvm_sM.ok;
+  assert  d.Void? ==> !lvm_sM.ok;
+  assert  !d.Void? ==> lvm_sM.ok;
+  assert  evalCode(lvm_b0.hd, lvm_s0, lvm_sM);
+  assert lvm_b0.hd == lvm_LOAD(dst,t,op1);
+  assert lvm_b0.hd.ins.LOAD?;
+  assert evalIns(lvm_b0.hd.ins,lvm_s0,lvm_sM);
+
+  assert lvm_b0.tl == lvm_bM;
+  assert lvm_sM.ok ==> !OperandContents(lvm_sM,dst).Ptr?;
+  assert lvm_sM.ok ==> OperandContents(lvm_sM,dst).Int? || OperandContents(lvm_sM,dst).Void?;
+  assert lvm_sM.ok ==> OperandContents(lvm_sM,dst).Int? ==> OperandContents(lvm_sM,dst).itype.size == t;
+  
+  assert lvm_sM.ok ==> ValidState(lvm_sM);
+  assert lvm_sM.ok ==> evalCode_lax(lvm_cM, lvm_s0, lvm_sM);
+  assert NextStep(lvm_s0,lvm_sM,evalInsStep(lvm_LOAD(dst,t,op1).ins));
+  assert MemStateNext(lvm_s0.m,lvm_sM.m,MemStep.stutterStep());
+  b' := b + [lvm_sM];
+  assert ValidBehavior(b');
+  assert BehaviorEvalsCode(lvm_LOAD(dst,t,op1),[lvm_s0,lvm_sM]);
+
+}
+
+
+
+function method lvm_code_ZEXT(dst:lvm_operand_opr,t:bitWidth,op1:lvm_operand_opr,dstSize:bitWidth):(out:lvm_code)
+    ensures out.Ins?;
+{
+    
+    Ins(ZEXT(dst,t,op1,dstSize))
+}
+
+lemma lvm_lemma_Zext(b:behavior,lvm_b0:lvm_codes, lvm_sN:lvm_state, 
+            dst:lvm_operand_opr, t:bitWidth,op1:lvm_operand_opr,dstSize:bitWidth)
+  returns (b':behavior,lvm_bM:lvm_codes, lvm_sM:lvm_state)
+
+   requires ValidBehaviorNonTrivial(b);
+  requires lvm_require(lvm_b0, lvm_code_ZEXT(dst,t,op1,dstSize), bls(b), lvm_sN)
+  requires lvm_is_dst_opr(dst, bls(b))
+  requires lvm_is_src_opr(op1, bls(b))
+  requires lvm_get_ok(bls(b))
+
+  requires ValidOperand(bls(b),op1);
+  requires ValidOperand(bls(b),dst);
+  requires OperandContents(bls(b),op1).Int?;
+  requires OperandContents(bls(b),op1).itype.size < dstSize;
+//   requires !OperandContents(bls(b),dst).itype.signed;
+
+// //   
+  ensures  lvm_ensure(lvm_b0, lvm_bM, bls(b), lvm_sM, lvm_sN)
+  ensures  lvm_get_ok(lvm_sM)
+  ensures  ValidOperand(lvm_sM,dst)
+  ensures  OperandContents(lvm_sM,dst).Int?;
+  ensures !OperandContents(lvm_sM,dst).itype.signed;
+  ensures  OperandContents(lvm_sM,dst).itype.size == dstSize;
+  ensures OperandContents(lvm_sM, dst).val == evalZEXT(OperandContents(bls(b),op1),dstSize).val;
+  ensures  lvm_state_eq(lvm_sM, lvm_update_ok(lvm_sM, lvm_update_all( lvm_sM, bls(b))))
+  ensures bls(b).m == lvm_sM.m;
+  ensures forall d :: ValidOperand(bls(b),d) && d != dst ==> ValidOperand(lvm_sM,d) && OperandContents(bls(b),d) == OperandContents(lvm_sM,d)
+  ensures StateNext(bls(b),lvm_sM)
+  ensures ValidBehavior(b');
+
+{
+    var lvm_s0 := bls(b);   
+    assert lvm_code_ZEXT(dst,t,op1,dstSize).Ins?;
+
+    assert ValidInstruction(lvm_s0, lvm_code_ZEXT(dst,t,op1,dstSize).ins);
+
+    ghost var lvm_ltmp1, lvm_cM:lvm_code, lvm_ltmp2 := lvm_lemma_block(lvm_b0, lvm_s0, lvm_sN);
+    lvm_sM := lvm_ltmp1;
+    lvm_bM := lvm_ltmp2;
+    // assert lvm_b0.tl == lvm_bM;
+    assert ValidState(lvm_s0);
+    // assert lvm_s0.ok;
+    assert ValidState(lvm_sM);
+    
+  assert lvm_sM.ok;
+  assert lvm_b0.tl == lvm_bM;
+
+  assert ValidState(lvm_sM);
+  assert evalCode_lax(lvm_cM, lvm_s0, lvm_sM);
+  assert NextStep(lvm_s0,lvm_sM,evalInsStep(lvm_code_ZEXT(dst,t,op1,dstSize).ins));
+  assert MemStateNext(lvm_s0.m,lvm_sM.m,MemStep.stutterStep());
+  b' := b + [lvm_sM];
+  assert ValidBehavior(b');
+  assert BehaviorEvalsCode(lvm_code_ZEXT(dst,t,op1,dstSize),[lvm_s0,lvm_sM]);
+}
+
+
+function method lvm_code_SEXT(dst:lvm_operand_opr,t:bitWidth,op1:lvm_operand_opr,dstSize:bitWidth):(out:lvm_code)
+    ensures out.Ins?;
+{
+    
+    Ins(SEXT(dst,t,op1,dstSize))
+}
+
+lemma lvm_lemma_Sext(b:behavior,lvm_b0:lvm_codes, lvm_sN:lvm_state, 
+            dst:lvm_operand_opr, t:bitWidth,op1:lvm_operand_opr,dstSize:bitWidth)
+  returns (b':behavior,lvm_bM:lvm_codes, lvm_sM:lvm_state)
+  requires ValidBehaviorNonTrivial(b);
+
+  requires lvm_require(lvm_b0, lvm_code_SEXT(dst,t,op1,dstSize), bls(b), lvm_sN)
+  requires lvm_is_dst_opr(dst, bls(b))
+  requires lvm_is_src_opr(op1, bls(b))
+  requires lvm_get_ok(bls(b))
+
+//   requires ValidInstruction(bls(b), lvm_code_ZEXT(dst,t,op1,dstSize).ins);
+  requires ValidOperand(bls(b),op1);
+  requires ValidOperand(bls(b),dst);
+  requires OperandContents(bls(b),op1).Int?;
+  requires OperandContents(bls(b),op1).itype.size < dstSize;
+  requires OperandContents(bls(b),dst).Int?;
+//   requires !OperandContents(bls(b),dst).itype.signed;
+
+// //   
+  ensures  lvm_ensure(lvm_b0, lvm_bM, bls(b), lvm_sM, lvm_sN)
+  ensures  lvm_get_ok(lvm_sM)
+  ensures  ValidOperand(lvm_sM,dst)
+  ensures  OperandContents(lvm_sM,dst).Int?;
+  ensures OperandContents(lvm_sM,dst).itype.signed;
+  ensures  OperandContents(lvm_sM,dst).itype.size == dstSize;
+  ensures OperandContents(lvm_sM, dst).val == evalSEXT(OperandContents(bls(b),op1),dstSize).val;
+  ensures  lvm_state_eq(lvm_sM, lvm_update_ok(lvm_sM, lvm_update_all( lvm_sM, bls(b))))
+  ensures forall d :: ValidOperand(bls(b),d) && d != dst ==> ValidOperand(lvm_sM,d) && OperandContents(bls(b),d) == OperandContents(lvm_sM,d)
+  ensures StateNext(bls(b),lvm_sM)
+    ensures ValidBehavior(b');
+
+
+{
+    var lvm_s0 := bls(b);
+    assert lvm_code_SEXT(dst,t,op1,dstSize).Ins?;
+
+    assert ValidInstruction(lvm_s0, lvm_code_SEXT(dst,t,op1,dstSize).ins);
+
+    ghost var lvm_ltmp1, lvm_cM:lvm_code, lvm_ltmp2 := lvm_lemma_block(lvm_b0, lvm_s0, lvm_sN);
+    lvm_sM := lvm_ltmp1;
+    lvm_bM := lvm_ltmp2;
+    // assert lvm_b0.tl == lvm_bM;
+    assert ValidState(lvm_s0);
+    // assert lvm_s0.ok;
+    assert ValidState(lvm_sM);
+   
+    assert lvm_sM.ok;
+    assert lvm_b0.tl == lvm_bM;
+
+    assert ValidState(lvm_sM);
+    assert evalCode_lax(lvm_cM, lvm_s0, lvm_sM);
+    assert NextStep(lvm_s0,lvm_sM,evalInsStep(lvm_code_SEXT(dst,t,op1,dstSize).ins));
+    assert MemStateNext(lvm_s0.m,lvm_sM.m,MemStep.stutterStep());
+    b' := b + [lvm_sM];
+    assert ValidBehavior(b');
+    assert BehaviorEvalsCode(lvm_code_SEXT(dst,t,op1,dstSize),[lvm_s0,lvm_sM]);
+
+}
+
+function method lvm_code_SHL(dst:lvm_operand_opr,src:lvm_operand_opr,shiftAmt:lvm_operand_opr):(out:lvm_code)
+    ensures out.Ins?;
+{
+    
+    Ins(SHL(dst,src,shiftAmt))
+}
+
+lemma lvm_lemma_Shl(b:behavior,lvm_b0:lvm_codes, lvm_sN:lvm_state, 
+            dst:lvm_operand_opr, src:lvm_operand_opr,shiftAmt:lvm_operand_opr)
+  returns (b':behavior,lvm_bM:lvm_codes, lvm_sM:lvm_state)
+
+  requires ValidBehaviorNonTrivial(b);
+
+  requires lvm_require(lvm_b0, lvm_code_SHL(dst,src,shiftAmt), bls(b), lvm_sN)
+  requires lvm_is_dst_opr(dst, bls(b))
+  requires lvm_is_src_opr(src, bls(b))
+  requires lvm_get_ok(bls(b))
+
+// is valid ins
+  requires ValidOperand(bls(b),src);
+  requires ValidOperand(bls(b),dst);
+  requires ValidOperand(bls(b),shiftAmt);
+
+  requires OperandContents(bls(b),src).Int?;
+  // requires OperandContents(bls(b),dst).Int?;
+  requires OperandContents(bls(b),shiftAmt).Int?;
+  requires OperandContents(bls(b),src).itype.size*8 > OperandContents(bls(b),shiftAmt).val
+  requires OperandContents(bls(b),shiftAmt).val > 0
+// //   
+  ensures  lvm_ensure(lvm_b0, lvm_bM, bls(b), lvm_sM, lvm_sN)
+  ensures  lvm_get_ok(lvm_sM)
+  ensures  ValidOperand(lvm_sM,dst)
+  ensures  ValidOperand(lvm_sM,src)
+
+  ensures  OperandContents(lvm_sM,dst).Int?;
+  ensures  OperandContents(lvm_sM,src).Int?;
+
+  ensures OperandContents(lvm_sM,dst).itype.size == OperandContents(lvm_sM,src).itype.size 
+  ensures OperandContents(lvm_sM,dst).itype.signed == OperandContents(lvm_sM,src).itype.signed
+  ensures OperandContents(lvm_sM, dst) == evalSHL(OperandContents(bls(b),src),OperandContents(bls(b),shiftAmt));
+  ensures  lvm_state_eq(lvm_sM, lvm_update_ok(lvm_sM, lvm_update_all( lvm_sM, bls(b))))
+  ensures bls(b).m == lvm_sM.m;
+  ensures forall d :: ValidOperand(bls(b),d) && d != dst ==> ValidOperand(lvm_sM,d) && OperandContents(bls(b),d) == OperandContents(lvm_sM,d)
+  ensures StateNext(bls(b),lvm_sM)
+    ensures ValidBehavior(b');
+
+
+{
+    var lvm_s0 := bls(b);
+    assert lvm_code_SHL(dst,src,shiftAmt).Ins?;
+
+    assert ValidInstruction(lvm_s0, lvm_code_SHL(dst,src,shiftAmt).ins);
+
+    ghost var lvm_ltmp1, lvm_cM:lvm_code, lvm_ltmp2 := lvm_lemma_block(lvm_b0, lvm_s0, lvm_sN);
+    lvm_sM := lvm_ltmp1;
+    lvm_bM := lvm_ltmp2;
+    assert ValidState(lvm_s0);
+    assert ValidState(lvm_sM);
+
+    assert lvm_sM.ok;
+    assert lvm_b0.tl == lvm_bM;
+
+    assert ValidState(lvm_sM);
+    assert evalCode_lax(lvm_cM, lvm_s0, lvm_sM);
+    assert NextStep(lvm_s0,lvm_sM,evalInsStep(lvm_code_SHL(dst,src,shiftAmt).ins));
+    assert MemStateNext(lvm_s0.m,lvm_sM.m,MemStep.stutterStep());
+    b' := b + [lvm_sM];
+    assert ValidBehavior(b');
+    assert BehaviorEvalsCode(lvm_code_SHL(dst,src,shiftAmt),[lvm_s0,lvm_sM]);
+
+}
+
+function method lvm_code_ICMP(dst:lvm_operand_opr,cond:lvm_cond,size:nat,op1:lvm_operand_opr,op2:lvm_operand_opr):(out:lvm_code)
+{
+    
+    Ins(ICMP(dst,cond,size,op1,op2))
+}
+
+lemma lvm_lemma_Icmp(b:behavior,lvm_b0:lvm_codes, lvm_sN:lvm_state,
+                    dst:lvm_operand_opr,cond:lvm_cond,size:nat,op1:lvm_operand_opr,op2:lvm_operand_opr)
+  returns (b':behavior,lvm_bM:lvm_codes, lvm_sM:lvm_state)
+
+  requires ValidBehaviorNonTrivial(b);
+
+  requires lvm_require(lvm_b0, lvm_code_ICMP(dst,cond,size,op1,op2), bls(b), lvm_sN)
+  requires lvm_is_dst_opr(dst, bls(b))
+  requires lvm_is_src_opr(op1, bls(b))
+  requires lvm_get_ok(bls(b))
+
+  requires lvm_code_ICMP(dst,cond,size,op1,op2).Ins?;
+  // requires ValidInstruction(bls(b),lvm_code_ICMP(dst,cond,size,op1,op2).ins);
+  requires ValidOperand(bls(b),dst) && ValidOperand(bls(b),op1) && ValidOperand(bls(b),op2);
+  requires OperandContents(bls(b),op1).Int?;
+  requires OperandContents(bls(b),op2).Int?;
+  requires typesMatch(OperandContents(bls(b),op1),OperandContents(bls(b),op2));
+  requires size == OperandContents(bls(b),op1).itype.size
+
+  ensures lvm_ensure(lvm_b0, lvm_bM, bls(b), lvm_sM, lvm_sN)
+  ensures lvm_get_ok(lvm_sM)
+  ensures ValidOperand(lvm_sM,dst)
+  ensures ValidOperand(lvm_sM,op1)
+  ensures OperandContents(lvm_sM,dst).Int?;
+  ensures OperandContents(lvm_sM,op1).Int?;
+  ensures OperandContents(bls(b),op1).itype == OperandContents(lvm_sM,op1).itype;
+  ensures !OperandContents(lvm_sM,dst).itype.signed
+  ensures OperandContents(lvm_sM,dst).itype.size == 1 
+
+  ensures OperandContents(lvm_sM, dst) == evalICMP(cond,size,OperandContents(bls(b),op1),OperandContents(bls(b),op2));
+  ensures lvm_state_eq(lvm_sM, lvm_update_ok(lvm_sM, lvm_update_all( lvm_sM, bls(b))))
+  ensures forall d :: ValidOperand(bls(b),d) && d != dst ==> ValidOperand(lvm_sM,d) && OperandContents(bls(b),d) == OperandContents(lvm_sM,d)
+  ensures StateNext(bls(b),lvm_sM)
+  ensures ValidBehavior(b');
+
+{
+    
+    var lvm_s0 := bls(b);
+
+    assert lvm_code_ICMP(dst,cond,size,op1,op2).Ins?;
+    assert ValidInstruction(lvm_s0,lvm_code_ICMP(dst,cond,size,op1,op2).ins);
+
+    ghost var lvm_ltmp1, lvm_cM:lvm_code, lvm_ltmp2 := lvm_lemma_block(lvm_b0, lvm_s0, lvm_sN);
+    lvm_sM := lvm_ltmp1;
+    lvm_bM := lvm_ltmp2;
+    assert ValidState(lvm_s0);
+    assert ValidState(lvm_sM);
+  
+    assert lvm_sM.ok;
+    assert lvm_b0.tl == lvm_bM;
+
+    assert ValidState(lvm_sM);
+    assert evalCode_lax(lvm_cM, lvm_s0, lvm_sM);
+    assert NextStep(lvm_s0,lvm_sM,evalInsStep(lvm_code_ICMP(dst,cond,size,op1,op2).ins));
+    assert MemStateNext(lvm_s0.m,lvm_sM.m,MemStep.stutterStep());
+    b' := b + [lvm_sM];
+    assert ValidBehavior(b');
+    assert BehaviorEvalsCode(lvm_code_ICMP(dst,cond,size,op1,op2),[lvm_s0,lvm_sM]);
+
+}
+
+function method lvm_code_Empty():lvm_code
+{   
+    lvm_Block(lvm_CNil())
+}       
+
+lemma lvm_lemma_Empty(b:behavior,lvm_b0:lvm_codes, lvm_sN:lvm_state)
+  returns (b':behavior,lvm_bM:lvm_codes, lvm_sM:lvm_state)
+  
+  requires ValidBehaviorNonTrivial(b);
+  requires lvm_require(lvm_b0, lvm_code_Empty(), bls(b), lvm_sN)
+  requires lvm_get_ok(bls(b))
+  ensures  lvm_ensure(lvm_b0, lvm_bM, bls(b), lvm_sM, lvm_sN)
+  ensures  lvm_get_ok(lvm_sM) // ValidState(sM)
+  ensures  lvm_state_eq(lvm_sM, bls(b))
+  ensures  lvm_state_eq(lvm_sM, lvm_update_mem( lvm_sM, lvm_update_ok(lvm_sM, lvm_sM)))
+  ensures  forall s2 :: evalCode(lvm_b0.hd, bls(b), s2) ==> s2.ok 
+  ensures StateNext(bls(b),lvm_sM)
+  ensures ValidBehavior(b');
+ 
+{
+    
+    var lvm_s0 := bls(b);
+
+    var lvm_old_s:lvm_state := lvm_s0;
+
+    assert lvm_s0.ok;
+    assert lvm_code_Empty() == Block(CNil);
+    assert lvm_b0.hd == lvm_code_Empty();
+    assert !lvm_b0.CNil?;
+    assert lvm_code_Empty().block.CNil?;
+    assert lvm_b0.hd.Block?;
+    assert lvm_get_block(lvm_b0.hd).CNil?;
+    assert evalBlock(lvm_get_block(lvm_b0.hd),lvm_s0, lvm_s0);
+    assert forall r :: r == lvm_s0 ==> eval_code(lvm_b0.hd,lvm_s0,r);
+    assert evalCode_lax(Block(lvm_b0), lvm_s0, lvm_sN);
+
+    // lvm_sM := lvm_lemma_empty(lvm_s0,lvm_sN);
+    ghost var lvm_ltmp1, lvm_cM:lvm_code, lvm_ltmp2 := lvm_lemma_block(lvm_b0, lvm_s0, lvm_sN);
+    lvm_sM := lvm_ltmp1;
+    lvm_bM := lvm_ltmp2;
+    var lvm_b1:lvm_codes := lvm_get_block(lvm_cM);
+
+    lvm_sM := lvm_lemma_empty(lvm_s0, lvm_sM);
+    assert ValidState(lvm_sM);
+    assert lvm_s0 == lvm_sM;
+    assert NextStep(lvm_s0,lvm_sM,Step.stutterStep());
+  assert MemStateNext(lvm_s0.m,lvm_sM.m,MemStep.stutterStep());
+  b' := b + [lvm_sM];
+  assert ValidBehavior(b');
+  assert BehaviorEvalsCode(lvm_code_Empty(),[lvm_s0,lvm_sM]);
+}
+
+function method lvm_code_ALLOCA(dst:lvm_operand_opr,t:bitWidth):(out:lvm_code)
+{
+    
+    Ins(ALLOCA(dst,t))
+}
+
+
+lemma lvm_lemma_Alloca(b:behavior,lvm_b0:lvm_codes, lvm_sN:lvm_state,dst:lvm_operand_opr,t:bitWidth)
+  returns (b':behavior,lvm_bM:lvm_codes, lvm_sM:lvm_state)
+  
+  requires ValidBehaviorNonTrivial(b);
+  requires lvm_require(lvm_b0, lvm_code_ALLOCA(dst,t), bls(b), lvm_sN)
+  requires lvm_get_ok(bls(b))
+  requires ValidOperand(bls(b),dst)
+  requires MemValid(bls(b).m)
+  requires OperandContents(bls(b),dst).Ptr?
+  requires validBitWidth(t)
+  ensures  lvm_ensure(lvm_b0, lvm_bM, bls(b), lvm_sM, lvm_sN)
+  ensures  lvm_get_ok(lvm_sM) // ValidState(sM)
+  ensures  lvm_state_eq(lvm_sM, lvm_update_mem( lvm_sM, lvm_update_ok(lvm_sM, lvm_sM)))
+  ensures  forall s2 :: evalCode(lvm_b0.hd, bls(b), s2) ==> s2.ok 
+  ensures StateNext(bls(b),lvm_sM)
+  ensures ValidBehaviorNonTrivial(b');
+  ensures  lvm_state_eq(lvm_sM, bls(b'))
+
+
+
+{
+    
+    var lvm_s0 := bls(b);
+    assert lvm_code_ALLOCA(dst,t).Ins?;
+
+    assert ValidInstruction(lvm_s0, lvm_code_ALLOCA(dst,t).ins);
+    assert evalBlock(lvm_b0, lvm_s0, lvm_sN);
+
+    // assert exists s',b :: (Alloc(lvm_s0.m,s'.m,b,t));
+    assert ValidState(lvm_s0) && lvm_s0.ok;
+    assert lvm_b0.hd.ins == lvm_code_ALLOCA(dst,t).ins;
+    assert lvm_b0.hd.Ins?;
+    // var s':MemState := AllocaStep(lvm_s0.m,t);
+    // var z:state := State(lvm_s0.lvs,lvm_s0.gvs,s',lvm_s0.ok);
+
+    // // && s'.mem == s.mem[s.nextBlock := UninitBlock(size)]
+    // assert ValidState(z); //&& Alloc(lvm_s0.m,s'.m,lvm_s0.m.nextBlock,t);
+    // assert Alloc(lvm_s0.m,z.m,lvm_s0.m.nextBlock,t);
+    // assert ValidData(z,evalALLOCA(lvm_s0.m,t));
+    // assert z == lvm_s0.(m := s'); 
+    // assert evalAlloca(lvm_s0, dst, t,z);
+    // // assert exists r':state :: evalIns(lvm_b0.hd.ins, lvm_s0, r') <==> evalCode(lvm_b0.hd, lvm_s0, r');
+    // assert evalIns(lvm_b0.hd.ins, lvm_s0, z);
+
+    // assert exists r':state :: evalCode(lvm_b0.hd, lvm_s0, r') && evalBlock(lvm_b0.tl, r', lvm_sN);
+    //              assert false;
+
+    // var r':state :| evalCode(lvm_b0.hd, lvm_s0, r') && evalBlock(lvm_b0.tl, r', lvm_sN);
+    //              assert false;
+
+    // assert lvm_b0.hd == lvm_code_ALLOCA(dst,t);
+    // assert evalIns(lvm_b0.hd.ins,lvm_s0,r');
+    
+    // assert r'.ok;
+    //      assert false;
+
+    ghost var lvm_ltmp1, lvm_cM:lvm_code, lvm_ltmp2 := lvm_lemma_block(lvm_b0, lvm_s0, lvm_sN);
+    lvm_sM := lvm_ltmp1;
+    lvm_bM := lvm_ltmp2;
+    assert ValidState(lvm_s0);
+    assert ValidState(lvm_sM);
+    //  assert false;
+
+    assert lvm_sM.ok;
+    assert lvm_b0.tl == lvm_bM;
+
+    assert ValidState(lvm_sM);
+    assert evalCode_lax(lvm_cM, lvm_s0, lvm_sM);
+    assert NextStep(lvm_s0,lvm_sM,evalInsStep(lvm_code_ALLOCA(dst,t).ins));
+    assert MemStateNext(lvm_s0.m,lvm_sM.m,MemStep.allocStep(lvm_s0.m.nextBlock,t));
+    b' := b + [lvm_sM];
+    assert ValidBehavior(b');
+    assert BehaviorEvalsCode(lvm_code_ALLOCA(dst,t),[lvm_s0,lvm_sM]);
+
+}
+
+function method lvm_code_CALL(dst:lvm_operand_opr,fnc:lvm_codes):(out:lvm_code)
+{
+    
+    Ins(CALL(dst,fnc))
+}
+
+lemma lvm_lemma_Call(b:behavior,lvm_b0:lvm_codes, lvm_sN:lvm_state,dst:lvm_operand_opr,fnc:lvm_codes)
+  returns (b':behavior,lvm_bM:lvm_codes, lvm_sM:lvm_state)
+  
+  requires ValidBehaviorNonTrivial(b);
+  requires lvm_require(lvm_b0, lvm_code_CALL(dst,fnc), bls(b), lvm_sN)
+  requires lvm_get_ok(bls(b))
+  requires ValidOperand(bls(b),dst)
+requires !fnc.CNil?;
+  ensures  lvm_ensure(lvm_b0, lvm_bM, bls(b), lvm_sM, lvm_sN)
+  ensures  lvm_get_ok(lvm_sM) // ValidState(sM)
+  ensures  lvm_state_eq(lvm_sM, lvm_update_mem( lvm_sM, lvm_update_ok(lvm_sM, lvm_sM)))
+  ensures  forall s2 :: evalCode(lvm_b0.hd, bls(b), s2) ==> s2.ok 
+  // ensures StateNext(bls(b),lvm_sM)
+  // ensures ValidBehaviorNonTrivial(b');
+  // ensures  lvm_state_eq(lvm_sM, bls(b'))
+
+
+
+{
+    
+    var lvm_s0 := bls(b);
+    assert lvm_code_CALL(dst,fnc).Ins?;
+
+    assert ValidInstruction(lvm_s0, lvm_code_CALL(dst,fnc).ins);
+    assert evalBlock(lvm_b0, lvm_s0, lvm_sN);
+
+    // assert exists s',b :: (Alloc(lvm_s0.m,s'.m,b,t));
+    assert ValidState(lvm_s0) && lvm_s0.ok;
+    assert lvm_b0.hd.ins == lvm_code_CALL(dst,fnc).ins;
+    assert lvm_b0.hd.Ins?;
+    // var s':MemState := AllocaStep(lvm_s0.m,t);
+
+
+    ghost var lvm_ltmp1, lvm_cM:lvm_code, lvm_ltmp2 := lvm_lemma_block(lvm_b0, lvm_s0, lvm_sN);
+    lvm_sM := lvm_ltmp1;
+    lvm_bM := lvm_ltmp2;
+    assert ValidState(lvm_s0);
+    assert ValidState(lvm_sM);
+    //  assert false;
+
+    assert lvm_sM.ok;
+    assert lvm_b0.tl == lvm_bM;
+
+    assert ValidState(lvm_sM);
+    // assert StateNext(lvm_s0,lvm_sM);
+    assert evalCode_lax(lvm_cM, lvm_s0, lvm_sM);
+    assert NextStep(lvm_s0,lvm_sM,evalInsStep(lvm_code_CALL(dst,fnc).ins));
+    // assert MemStateNext(lvm_s0.m,lvm_sM.m,MemStep.allocStep(lvm_s0.m.nextBlock,t));
+    b' := b + [lvm_sM];
+    assert lvm_state_eq(lvm_sM, bls(b'));
+    // assert ValidBehavior(b');
+    assert BehaviorEvalsCode(lvm_code_CALL(dst,fnc),[lvm_s0,lvm_sM]);
+
+}
+
+function method lvm_code_MEMCPY(dst:lvm_operand_opr,src:lvm_operand_opr,len:bitWidth):(out:lvm_code)
+{
+    
+    Ins(LLVM_MEMCPY(dst,src,len,false))
+}
+
+
+
+lemma lvm_lemma_MemCpy(b:behavior,lvm_b0:lvm_codes, lvm_sN:lvm_state,dst:lvm_operand_opr,src:lvm_operand_opr,len:bitWidth)
+  returns (b':behavior,lvm_bM:lvm_codes, lvm_sM:lvm_state)
+  
+  requires ValidBehaviorNonTrivial(b);
+  requires lvm_require(lvm_b0, lvm_code_MEMCPY(dst,src,len), bls(b), lvm_sN)
+  requires lvm_get_ok(bls(b))
+  requires ValidOperand(bls(b),dst)
+  requires ValidOperand(bls(b),src)
+  requires MemValid(bls(b).m)
+  requires OperandContents(bls(b),dst).Ptr?
+  requires OperandContents(bls(b),src).Ptr?
+  requires OperandContents(bls(b),dst).size >= OperandContents(bls(b),src).size;
+  requires validBitWidth(len)
+  ensures  lvm_ensure(lvm_b0, lvm_bM, bls(b), lvm_sM, lvm_sN)
+  ensures  lvm_get_ok(lvm_sM) // ValidState(sM)
+  ensures  lvm_state_eq(lvm_sM, lvm_update_mem( lvm_sM, lvm_update_ok(lvm_sM, lvm_sM)))
+  ensures  forall s2 :: evalCode(lvm_b0.hd, bls(b), s2) ==> s2.ok 
+  ensures StateNext(bls(b),lvm_sM)
+  ensures ValidBehaviorNonTrivial(b');
+  ensures  lvm_state_eq(lvm_sM, bls(b'))
+
+
+
+{
+    
+    var lvm_s0 := bls(b);
+    assert lvm_code_MEMCPY(dst,src,len).Ins?;
+
+    assert ValidInstruction(lvm_s0, lvm_code_MEMCPY(dst,src,len).ins);
+    assert evalBlock(lvm_b0, lvm_s0, lvm_sN);
+
+    // assert exists s',b :: (Alloc(lvm_s0.m,s'.m,b,t));
+    assert ValidState(lvm_s0) && lvm_s0.ok;
+    assert lvm_b0.hd.ins == lvm_code_MEMCPY(dst,src,len).ins;
+    assert lvm_b0.hd.Ins?;
+   
+
+    ghost var lvm_ltmp1, lvm_cM:lvm_code, lvm_ltmp2 := lvm_lemma_block(lvm_b0, lvm_s0, lvm_sN);
+    lvm_sM := lvm_ltmp1;
+    lvm_bM := lvm_ltmp2;
+    assert ValidState(lvm_s0);
+    assert ValidState(lvm_sM);
+    //  assert false;
+
+    assert lvm_sM.ok;
+    assert lvm_b0.tl == lvm_bM;
+
+    assert ValidState(lvm_sM);
+    assert evalCode_lax(lvm_cM, lvm_s0, lvm_sM);
+    assert NextStep(lvm_s0,lvm_sM,evalInsStep(lvm_code_MEMCPY(dst,src,len).ins));
+    // assert MemStateNext(lvm_s0.m,lvm_sM.m,MemStep.allocStep(lvm_s0.m.nextBlock,t));
+    b' := b + [lvm_sM];
+    assert ValidBehavior(b');
+    assert BehaviorEvalsCode(lvm_code_MEMCPY(dst,src,len),[lvm_s0,lvm_sM]);
+
+}
+
+}
